functional spec and correctness statement of strotimax

asn_strtoimax_lim_spec.v
@@ -2,8 +2,10 @@ From Coq Require Import String List ZArith Psatz.
 From compcert Require Import Coqlib Integers Floats AST Ctypes Cop Clight Clightdefs Memory Values ClightBigstep Events Maps.
 Local Open Scope Z_scope.
 Import ListNotations.
+Require Import StructTact.StructTactics.
 
-(* Notations for integers *)
+
+(* Notations for integers and ptrofs *)
 
 Delimit Scope IntScope with int.
 Infix "==" := Int.eq (at level 70) : IntScope.
@@ -15,9 +17,24 @@ Infix "+" := Int.add : IntScope.
 Infix "-" := Int.sub : IntScope.
 Infix "*" := Int.mul : IntScope.
 Infix "<" := Int.lt : IntScope.
-Notation "x <= y" := (negb (Int.lt y x)) (at level 70) : IntScope.
+Notation "x <= y" := (negb (Int.ltu y x)) (at level 70) : IntScope.
 Infix "%" := Int.mods (at level 70) : IntScope.
 Infix "//" := Int.divs (at level 70) : IntScope.
+
+Delimit Scope PtrofsScope with ptrofs.
+Infix "==" := Ptrofs.eq (at level 70) : PtrofsScope.
+Notation "x ~= y" := (negb Ptrofs.eq x y) (at level 70) : PtrofsScope.
+Notation "x >> y" := (Ptrofs.shru x y) (at level 70) : PtrofsScope.
+Notation "0" := Ptrofs.zero : PtrofsScope.
+Notation "1" := Ptrofs.one : PtrofsScope.
+Infix "+" := Ptrofs.add : PtrofsScope.
+Infix "-" := Ptrofs.sub : PtrofsScope.
+Infix "*" := Ptrofs.mul : PtrofsScope.
+Infix "<" := Ptrofs.lt : PtrofsScope.
+Notation "x <= y" := (negb (Ptrofs.ltu y x)) (at level 70) : PtrofsScope.
+Infix "%" := Ptrofs.mods (at level 70) : PtrofsScope.
+Infix "//" := Ptrofs.divs (at level 70) : PtrofsScope.
+
 Local Open Scope IntScope.
 
 (* Functional specification of INTEGER.asn_strtoimax_lim
@@ -51,10 +68,40 @@ Parameter e : env.
 Parameter le : temp_env.
 
 (* Pointer comparison *)
-Definition ptr_ge (a1 a2: addr) : option bool :=
- match a1,a2 with (b1,ofs1), (b2,ofs2) =>
-                  if Archi.ptr64                                                   then Val.cmplu_bool (Mem.valid_pointer m) Cge (Vptr b1 ofs1) (Vptr b2 ofs2)                                                       else Val.cmpu_bool (Mem.valid_pointer m) Cge (Vptr b1 ofs1) (Vptr b2 ofs2)
- end.
+
+(* Abstract spec *)
+
+(* [b1,ofs1] >= [b2,ofs2] *)
+Definition ptr_ge_spec (b1 b2 : block) (ofs1 ofs2 : ptrofs) :=
+  if eq_block b1 b2 then Some (ofs2 <= ofs1)%ptrofs else None.
+
+(* Concrete spec using Compcert semantic values *)
+
+Definition ptr_ge (b1 b2 : block) (ofs1 ofs2 : ptrofs) := if Archi.ptr64
+  then Val.cmplu_bool (Mem.valid_pointer m) Cge (Vptr b1 ofs1) (Vptr b2 ofs2)                        else Val.cmpu_bool (Mem.valid_pointer m) Cge (Vptr b1 ofs1) (Vptr b2 ofs2).
+
+
+Proposition ptr_ge_refine : forall (b1 b2 : block) (ofs1 ofs2 : ptrofs),
+    Mem.weak_valid_pointer m b1 (Ptrofs.unsigned ofs1) = true ->
+    Mem.weak_valid_pointer m b2 (Ptrofs.unsigned ofs2) = true ->
+    
+    ptr_ge_spec b1 b2 ofs1 ofs2 = ptr_ge b1 b2 ofs1 ofs2.
+Proof.
+  intros.
+  unfold ptr_ge.
+  simpl; unfold Mem.weak_valid_pointer in *.
+  destruct Archi.ptr64 eqn: A; simpl.
+  all: rewrite H;
+    rewrite H0;
+    simpl;
+    destruct (Mem.valid_pointer m b1 (Ptrofs.unsigned ofs1) &&
+                                Mem.valid_pointer m b2 (Ptrofs.unsigned ofs2));
+    auto.
+Qed.
+
+
+
+Definition addr_ge (a1 a2 : addr) := match a1, a2 with (b1,ofs1), (b2,ofs2) => ptr_ge b1 b2 ofs1 ofs2 end.
 
 Definition _end : ident := 152%positive.
 Definition _str : ident := 151%positive.
@@ -65,50 +112,13 @@ Definition f_ptr_ge := (Sifthenelse (Ebinop Oge (Etempvar _str (tptr tschar))
             (Sreturn (Some (Econst_int (Int.repr (-2)) tint)))
             Sskip).
 
-(** [break_if] finds instances of [if _ then _ else _] in your goal or
-    context, and destructs the discriminee, while retaining the
-    information about the discriminee's value leading to the branch
-    being taken. *)
-Ltac break_if :=
-  match goal with
-    | [ |- context [ if ?X then _ else _ ] ] =>
-      match type of X with
-        | sumbool _ _ => destruct X
-        | _ => destruct X eqn:?
-      end
-    | [ H : context [ if ?X then _ else _ ] |- _] =>
-      match type of X with
-        | sumbool _ _ => destruct X
-        | _ => destruct X eqn:?
-      end
-  end.
-
-(** [break_let] breaks a destructuring [let] for a pair. *)
-Ltac break_let :=
-  match goal with
-    | [ H : context [ (let (_,_) := ?X in _) ] |- _ ] => destruct X eqn:?
-    | [ |- context [ (let (_,_) := ?X in _) ] ] => destruct X eqn:?
-end.
-
-Ltac break_match_hyp :=
-  match goal with
-    | [ H : context [ match ?X with _ => _ end ] |- _] =>
-      match type of X with
-        | sumbool _ _ => destruct X
-        | _ => destruct X eqn:?
-      end
-  end.
-
-Proposition ptr_ge_corr : forall a1 a2, ptr_ge a1 a2 = Some true -> exists t le',
-      le!_str = Some (Vptr (fst a1) (snd a1)) ->
-      le!_end = Some (Vptr (fst a2) (snd a2)) ->                  
+Proposition ptr_ge_corr : forall b1 b2 ofs1 ofs2, ptr_ge b1 b2 ofs1 ofs2 = Some true ->
+                                             exists t le', le!_str = Some (Vptr b1 ofs1) ->
+                                                      le!_end = Some (Vptr b2 ofs2) ->                  
       exec_stmt ge e le m f_ptr_ge t le' m (Out_return (Some (Vint (Int.repr (-2)),tint))).
 Proof.
-  intros str fin Spec.
-   unfold ptr_ge in Spec.
-  (*assert (Archi.ptr64 = false) as A by (simpl; auto); rewrite A in Spec. *)
-  repeat break_let.
-  (* repeat break_if. subst. *)
+  intros until ofs2; intro Spec.
+  unfold ptr_ge in Spec.
   repeat eexists.
   intros Fin Str.
   repeat econstructor.
@@ -118,22 +128,12 @@ Proof.
   unfold sem_cmp.
   simpl.
   unfold cmp_ptr.
-  pose (option_map Val.of_bool (if Archi.ptr64
-          then
-           Val.cmplu_bool (Mem.valid_pointer m) Cge 
-             (Vptr b i) (Vptr b0 i0)
-          else
-           Val.cmpu_bool (Mem.valid_pointer m) Cge 
-             (Vptr b i) (Vptr b0 i0))).
-    assert ( (option_map Val.of_bool (if Archi.ptr64
-          then
-           Val.cmplu_bool (Mem.valid_pointer m) Cge 
-             (Vptr b i) (Vptr b0 i0)
-          else
-           Val.cmpu_bool (Mem.valid_pointer m) Cge 
-                         (Vptr b i) (Vptr b0 i0))) = (option_map Val.of_bool (Some true))).
-    f_equal.
-    assumption.
+  assert (option_map Val.of_bool
+    (if Archi.ptr64
+     then Val.cmplu_bool (Mem.valid_pointer m) Cge (Vptr b1 ofs1) (Vptr b2 ofs2)
+     else Val.cmpu_bool (Mem.valid_pointer m) Cge (Vptr b1 ofs1) (Vptr b2 ofs2)) = (option_map Val.of_bool (Some true))).
+  f_equal.
+  assumption.
     eapply H.
     simpl.
     econstructor.
@@ -141,9 +141,8 @@ Proof.
     econstructor.
     Qed.
     
-(* we are reading a char type from the memory *)
+(* We are reading a char type from the memory *)
 Definition chunk := Mint8signed : memory_chunk.
-
 Definition load_addr (m : mem) (a : addr) := match a with (b,ofs) =>  Mem.loadv chunk m (Vptr b ofs) end.
 Definition next_addr (a : addr) := match a with (b,ofs) => (b, Ptrofs.add ofs Ptrofs.one) end.
 Notation "a ++" := (next_addr a) (at level 20).
@@ -152,52 +151,287 @@ Notation plus_char := (Int.repr 43).
 Notation zero_char := (Int.repr 48).
 
 Definition ASN1_INTMAX_MAX :=(Int.not 0) >> 1.
-Definition upper_boundary := ASN1_INTMAX_MAX // (Int.repr 10).
-Definition last_digit_max_plus := ASN1_INTMAX_MAX % (Int.repr 10).
-Definition last_digit_max_minus := (ASN1_INTMAX_MAX % (Int.repr 10)) + 1.
-(* [0-9]*)
-Definition digits := map Int.repr [48;49;50;51;52;53;54;55;56;57].
-Definition distance (a1 a2 : addr) : nat :=
-  ((Z.to_nat (Ptrofs.unsigned (snd a1))) - (Z.to_nat (Ptrofs.unsigned (snd a1))))%nat.
 
-(* The spec close to C code *)
-
-Program Fixpoint asn_strtoimax_lim_loop (str : addr) (fin : addr) (value : int) (s: signedness) (last_digit_m : int) {measure (distance str fin) } : option (asn_strtox_result_e*addr*int*signedness)  :=
-  if Nat.eq_dec (distance str fin) O then Some (ASN_STRTOX_OK, str, value, s) else
-  match load_addr m str with
-  | Some (Vint i) => if existsb (fun j => Int.eq i j) digits then
-                      let d := i - zero_char in
-                      let v := (value*(Int.repr 10) + d) in
-                      if value < upper_boundary then asn_strtoimax_lim_loop (str++) fin v s last_digit_m
-                      else if (value == upper_boundary) && (d <= last_digit_m)
-                           then  asn_strtoimax_lim_loop (str++) fin v s last_digit_m
-                           else Some (ASN_STRTOX_ERROR_RANGE,str,value,s) 
-                      else Some (ASN_STRTOX_EXTRA_DATA, str,value,s)
-  | _  => None (* fail of memory load: wrong type or not enough permission *)
-  end.
-Admit Obligations.
-
-Definition asn_strtoimax_lim (str fin : addr) (last_digit_max: int) : option (asn_strtox_result_e*addr*int*signedness) :=
-  match ptr_ge str fin with
-  | Some true => None (* error *)
-  | Some false => match load_addr m str with
-                 | Some (Vint i) =>
-                   if (i == minus_char)
-                   then asn_strtoimax_lim_loop (str++) fin 0 Signed (last_digit_max + 1)
-                   else if (i == plus_char)
-                        then asn_strtoimax_lim_loop (str++) fin 0 Unsigned last_digit_max
-                        else asn_strtoimax_lim_loop str fin 0 Unsigned last_digit_max                      
-                 | _ => None (* fail of memory load: wrong type or not enough permission *)
-                 end
-  | None => None (* error in pointer comparison *)
-  end.
-
-
-  
 Fact shift_pow2_div :  (Int64.shru (Int64.not Int64.zero) Int64.one) = Int64.repr (Int64.max_unsigned / 2).
   replace (Int64.not Int64.zero) with (Int64.repr Int64.max_unsigned) by (auto with ints).
   unfold Int64.shru.
   f_equal.
   Qed.
+
+Definition upper_boundary := ASN1_INTMAX_MAX // (Int.repr 10).
+Definition last_digit_max_plus := ASN1_INTMAX_MAX % (Int.repr 10).
+Definition last_digit_max_minus := (ASN1_INTMAX_MAX % (Int.repr 10)) + 1.
+(* [0-9]*)
+Definition digits := map Int.repr [48;49;50;51;52;53;54;55;56;57].
+
+Definition distance (a1 a2 : addr) : nat :=
+  ((Z.to_nat (Ptrofs.unsigned (snd a1))) - (Z.to_nat (Ptrofs.unsigned (snd a1))))%nat.
+
+(* Functional spec *)
+
+Fixpoint asn_strtoimax_lim_loop (str : addr) (fin : addr) (value : int) (s: signedness) (last_digit : int) (dist : nat) {struct dist} : option (asn_strtox_result_e*option (addr*int*signedness))  :=
+   match dist with
+   | O => Some (ASN_STRTOX_OK, Some (str, value, s))
+   | S n => match load_addr m str with
+           | Some (Vint i) => if existsb (fun j => Int.eq i j) digits then
+                      let d := i - zero_char in
+                      let v := (value*(Int.repr 10) + d) in
+                      if value < upper_boundary
+                      then asn_strtoimax_lim_loop (str++) fin v s last_digit n
+                      else if (value == upper_boundary) && (d <= last_digit)
+                           then asn_strtoimax_lim_loop (str++) fin v s last_digit n
+                           else Some (ASN_STRTOX_ERROR_RANGE, Some (str,value,s)) 
+                      else Some (ASN_STRTOX_EXTRA_DATA, Some (str,value,s))
+           | _  => None (* fail of memory load: wrong type or not enough permission *)
+            end
+  end.
+
+Definition asn_strtoimax_lim (str fin : addr) : option (asn_strtox_result_e*(option(addr*int*signedness))) :=
+  match addr_ge str fin with (* compare str and fin *)
+  | Some true => Some (ASN_STRTOX_ERROR_INVAL, None)
+  | Some false => let dist := distance str fin in
+                 match load_addr m str with
+                 | Some (Vint i) =>
+                   if (i == minus_char)
+                   then asn_strtoimax_lim_loop (str++) fin 0 Signed last_digit_max_minus dist
+                   else if (i == plus_char)
+                        then asn_strtoimax_lim_loop (str++) fin 0 Unsigned last_digit_max_plus dist
+                        else asn_strtoimax_lim_loop str fin 0 Unsigned last_digit_max_plus dist
+                 | _ => None (* fail of memory load on str: wrong type or not enough permission *)
+                 end
+  | None => None (* error in pointer comparison *)
+  end.
+
+Definition _last_digit_max : ident := 155%positive.
+Definition _upper_boundary : ident := 155%positive.
+Definition _value : ident := 29%positive.
+Definition _t'1 : ident := 160%positive.
+Definition _t'2 : ident := 161%positive.
+Definition _t'3 : ident := 162%positive.
+Definition _t'4 : ident := 163%positive.
+Definition _t'5 : ident := 164%positive.
+Definition _sign : ident := 168%positive.
+Definition _intp : ident := 169%positive.
+Definition _d : ident := 170%positive.
+
+
+Definition f_asn_strtoimax_lim := {|
+  fn_return := tint;
+  fn_callconv := cc_default;
+  fn_params := ((_str, (tptr tschar)) :: (_end, (tptr (tptr tschar))) ::
+                (_intp, (tptr tlong)) :: nil);
+  fn_vars := nil;
+  fn_temps := ((_sign, tint) :: (_value, tlong) ::
+               (_upper_boundary, tlong) :: (_last_digit_max, tlong) ::
+               (_d, tint) :: (_t'6, (tptr tschar)) ::
+               (_t'5, (tptr tschar)) :: (_t'4, tschar) ::
+               (_t'3, (tptr tschar)) :: (_t'2, tschar) :: (_t'1, tschar) ::
+               nil);
+  fn_body :=
+(Ssequence
+  (Sset _sign (Econst_int (Int.repr 1) tint))
+  (Ssequence
+    (Sset _upper_boundary
+      (Ebinop Odiv
+        (Ebinop Oshr
+          (Eunop Onotint (Ecast (Econst_int (Int.repr 0) tint) tulong)
+            tulong) (Econst_int (Int.repr 1) tint) tulong)
+        (Econst_int (Int.repr 10) tint) tulong))
+    (Ssequence
+      (Sset _last_digit_max
+        (Ebinop Omod
+          (Ebinop Oshr
+            (Eunop Onotint (Ecast (Econst_int (Int.repr 0) tint) tulong)
+              tulong) (Econst_int (Int.repr 1) tint) tulong)
+          (Econst_int (Int.repr 10) tint) tulong))
+      (Ssequence
+        (Ssequence
+          (Sset _t'6
+            (Ederef (Etempvar _end (tptr (tptr tschar))) (tptr tschar)))
+          (Sifthenelse (Ebinop Oge (Etempvar _str (tptr tschar))
+                         (Etempvar _t'6 (tptr tschar)) tint)
+            (Sreturn (Some (Econst_int (Int.repr (-2)) tint)))
+            Sskip))
+        (Ssequence
+          (Ssequence
+            (Sset _t'4 (Ederef (Etempvar _str (tptr tschar)) tschar))
+            (Sswitch (Ederef (Etempvar _str (tptr tschar)) tschar)
+              (LScons (Some 45)
+                (Ssequence
+                  (Sset _last_digit_max
+                    (Ebinop Oadd (Etempvar _last_digit_max tlong)
+                      (Econst_int (Int.repr 1) tint) tlong))
+                  (Sset _sign
+                    (Eunop Oneg (Econst_int (Int.repr 1) tint) tint)))
+                (LScons (Some 43)
+                  (Ssequence
+                    (Sset _str
+                      (Ebinop Oadd (Etempvar _str (tptr tschar))
+                        (Econst_int (Int.repr 1) tint) (tptr tschar)))
+                    (Ssequence
+                      (Sset _t'5
+                        (Ederef (Etempvar _end (tptr (tptr tschar)))
+                          (tptr tschar)))
+                      (Sifthenelse (Ebinop Oge (Etempvar _str (tptr tschar))
+                                     (Etempvar _t'5 (tptr tschar)) tint)
+                        (Ssequence
+                          (Sassign
+                            (Ederef (Etempvar _end (tptr (tptr tschar)))
+                              (tptr tschar)) (Etempvar _str (tptr tschar)))
+                          (Sreturn (Some (Econst_int (Int.repr (-1)) tint))))
+                        Sskip)))
+                  LSnil))))
+          (Ssequence
+            (Ssequence
+              (Sset _value (Ecast (Econst_int (Int.repr 0) tint) tlong))
+              (Sloop
+                (Ssequence
+                  (Ssequence
+                    (Sset _t'3
+                      (Ederef (Etempvar _end (tptr (tptr tschar)))
+                        (tptr tschar)))
+                    (Sifthenelse (Ebinop Olt (Etempvar _str (tptr tschar))
+                                   (Etempvar _t'3 (tptr tschar)) tint)
+                      Sskip
+                      Sbreak))
+                  (Ssequence
+                    (Sset _t'1 (Ederef (Etempvar _str (tptr tschar)) tschar))
+                    (Sswitch (Ederef (Etempvar _str (tptr tschar)) tschar)
+                      (LScons (Some 48)
+                        Sskip
+                        (LScons (Some 49)
+                          Sskip
+                          (LScons (Some 50)
+                            Sskip
+                            (LScons (Some 51)
+                              Sskip
+                              (LScons (Some 52)
+                                Sskip
+                                (LScons (Some 53)
+                                  Sskip
+                                  (LScons (Some 54)
+                                    Sskip
+                                    (LScons (Some 55)
+                                      Sskip
+                                      (LScons (Some 56)
+                                        Sskip
+                                        (LScons (Some 57)
+                                          (Ssequence
+                                            (Ssequence
+                                              (Sset _t'2
+                                                (Ederef
+                                                  (Etempvar _str (tptr tschar))
+                                                  tschar))
+                                              (Sset _d
+                                                (Ebinop Osub
+                                                  (Etempvar _t'2 tschar)
+                                                  (Econst_int (Int.repr 48) tint)
+                                                  tint)))
+                                            (Ssequence
+                                              (Sifthenelse (Ebinop Olt
+                                                             (Etempvar _value tlong)
+                                                             (Etempvar _upper_boundary tlong)
+                                                             tint)
+                                                (Sset _value
+                                                  (Ebinop Oadd
+                                                    (Ebinop Omul
+                                                      (Etempvar _value tlong)
+                                                      (Econst_int (Int.repr 10) tint)
+                                                      tlong)
+                                                    (Etempvar _d tint) tlong))
+                                                (Sifthenelse (Ebinop Oeq
+                                                               (Etempvar _value tlong)
+                                                               (Etempvar _upper_boundary tlong)
+                                                               tint)
+                                                  (Sifthenelse (Ebinop Ole
+                                                                 (Etempvar _d tint)
+                                                                 (Etempvar _last_digit_max tlong)
+                                                                 tint)
+                                                    (Sifthenelse (Ebinop Ogt
+                                                                   (Etempvar _sign tint)
+                                                                   (Econst_int (Int.repr 0) tint)
+                                                                   tint)
+                                                      (Sset _value
+                                                        (Ebinop Oadd
+                                                          (Ebinop Omul
+                                                            (Etempvar _value tlong)
+                                                            (Econst_int (Int.repr 10) tint)
+                                                            tlong)
+                                                          (Etempvar _d tint)
+                                                          tlong))
+                                                      (Ssequence
+                                                        (Sset _sign
+                                                          (Econst_int (Int.repr 1) tint))
+                                                        (Sset _value
+                                                          (Ebinop Osub
+                                                            (Ebinop Omul
+                                                              (Eunop Oneg
+                                                                (Etempvar _value tlong)
+                                                                tlong)
+                                                              (Econst_int (Int.repr 10) tint)
+                                                              tlong)
+                                                            (Etempvar _d tint)
+                                                            tlong))))
+                                                    (Ssequence
+                                                      (Sassign
+                                                        (Ederef
+                                                          (Etempvar _end (tptr (tptr tschar)))
+                                                          (tptr tschar))
+                                                        (Etempvar _str (tptr tschar)))
+                                                      (Sreturn (Some (Econst_int (Int.repr (-3)) tint)))))
+                                                  (Ssequence
+                                                    (Sassign
+                                                      (Ederef
+                                                        (Etempvar _end (tptr (tptr tschar)))
+                                                        (tptr tschar))
+                                                      (Etempvar _str (tptr tschar)))
+                                                    (Sreturn (Some (Econst_int (Int.repr (-3)) tint))))))
+                                              Scontinue))
+                                          (LScons None
+                                            (Ssequence
+                                              (Sassign
+                                                (Ederef
+                                                  (Etempvar _end (tptr (tptr tschar)))
+                                                  (tptr tschar))
+                                                (Etempvar _str (tptr tschar)))
+                                              (Ssequence
+                                                (Sassign
+                                                  (Ederef
+                                                    (Etempvar _intp (tptr tlong))
+                                                    tlong)
+                                                  (Ebinop Omul
+                                                    (Etempvar _sign tint)
+                                                    (Etempvar _value tlong)
+                                                    tlong))
+                                                (Sreturn (Some (Econst_int (Int.repr 1) tint)))))
+                                            LSnil))))))))))))))
+                (Sset _str
+                  (Ebinop Oadd (Etempvar _str (tptr tschar))
+                    (Econst_int (Int.repr 1) tint) (tptr tschar)))))
+            (Ssequence
+              (Sassign
+                (Ederef (Etempvar _end (tptr (tptr tschar))) (tptr tschar))
+                (Etempvar _str (tptr tschar)))
+              (Ssequence
+                (Sassign (Ederef (Etempvar _intp (tptr tlong)) tlong)
+                  (Ebinop Omul (Etempvar _sign tint) (Etempvar _value tlong)
+                    tlong))
+                (Sreturn (Some (Econst_int (Int.repr 0) tint)))))))))))
+                                 |}.
+
+Definition vptr (a : addr) := match a with (b,ofs) => Vptr b ofs end.
+
+Theorem asn_strtoimax_lim_correct : forall str fin value, 
+    asn_strtoimax_lim str fin = Some (ASN_STRTOX_OK, Some (str, value, Unsigned)) ->
+    exists t le', le!_str = Some (vptr str)  ->
+             le!_end = Some (vptr fin) ->
+      
+             exec_stmt ge e le m f_asn_strtoimax_lim.(fn_body) t le' m (Out_return (Some (Vint (asn_strtox_result_e_to_int ASN_STRTOX_OK), tint)))
+             /\ le'!_intp = Some (Vint value)
+             /\ le'!_end = Some (vptr str).
+  
+              
+
+
 
 
